backend/Allocproof.v
@@ -2526,7 +2526,7 @@ Proof.
   intros. inv H.
   exploit function_ptr_translated; eauto. intros [tf [FIND TR]].
   exploit sig_function_translated; eauto. intros SIG.
-  exists (LTL.Callstate nil tf (Locmap.init Vundef) m0 (prog_main tprog)); split.
+  exists (LTL.Callstate nil tf (Locmap.init Vundef) m1 (prog_main tprog)); split.
   econstructor; eauto.
   eapply (Genv.init_mem_transf_partial TRANSF); eauto.
   rewrite symbols_preserved.
